Regex/NFA/Compile.lean
@@ -4,6 +4,282 @@ import Regex.NFA.Basic
 
 import Std.Data.Array.Lemmas
 
+namespace NFAa
+
+-- TODO: remove once migration is complete
+open NFA
+
+def pushNode (nfa : NFAa) (node : NFA.Node) (inBounds : node.inBounds (nfa.nodes.size + 1)) :
+  { nfa' : NFAa // nfa.nodes.size < nfa'.nodes.size } :=
+  let start := nfa.nodes.size
+  let nodes := nfa.nodes.push node
+  have inBounds := by
+    intro i
+    simp
+    rw [Array.get_push]
+    split
+    case inl h =>
+      have := nfa.inBounds ⟨i.val, h⟩
+      apply Node.inBounds_of_inBounds_of_le this (Nat.le_succ _)
+    case inr => exact inBounds
+  let nfa' : NFAa := ⟨nodes, ⟨start, by simp⟩, inBounds⟩
+
+  ⟨nfa', by simp⟩
+
+@[simp]
+theorem pushNode_size {nfa : NFAa} {node : Node} {inBounds : node.inBounds (nfa.nodes.size + 1)} :
+  (nfa.pushNode node inBounds).val.nodes.size = nfa.nodes.size + 1 := by
+  simp [pushNode]
+
+theorem pushNode_get_lt {nfa : NFAa} {node : Node} {inBounds : node.inBounds (nfa.nodes.size + 1)}
+  (i : Nat) (h : i < nfa.nodes.size) :
+  (nfa.pushNode node inBounds).val[i]'(Nat.lt_trans h (nfa.pushNode node inBounds).property) = nfa[i] := by
+  simp [pushNode, get_eq_nodes_get]
+  rw [Array.get_push_lt]
+
+@[simp]
+theorem pushNode_get_eq {nfa : NFAa} {node : Node} {inBounds : node.inBounds (nfa.nodes.size + 1)} :
+  (nfa.pushNode node inBounds).val[nfa.nodes.size] = node := by
+  simp [pushNode, get_eq_nodes_get]
+
+theorem pushNode_get {nfa : NFAa} {node : Node} {inBounds : node.inBounds (nfa.nodes.size + 1)}
+  (i : Nat) (h : i < (nfa.pushNode node inBounds).val.nodes.size) :
+  (nfa.pushNode node inBounds).val[i]'h = if h' : i < nfa.nodes.size then nfa[i]'h' else node := by
+  simp at h
+  cases Nat.lt_or_eq_of_le (Nat.le_of_succ_le_succ h) with
+  | inl lt => simp [lt, pushNode_get_lt _ lt]
+  | inr eq => simp [eq]
+
+@[simp]
+theorem pushNode_start_eq {nfa : NFAa} {node : Node} {inBounds : node.inBounds (nfa.nodes.size + 1)} :
+  (nfa.pushNode node inBounds).val.start.val = nfa.nodes.size := rfl
+
+/--
+  Compile a Regex and append the resulting nodes to the NFA. The nodes will transition to `next` on match.
+-/
+def pushRegex (nfa : NFAa) (next : Fin nfa.nodes.size) :
+  Regex → { nfa' : NFAa // nfa.nodes.size < nfa'.nodes.size }
+  | .empty => nfa.pushNode .fail rfl
+  | .epsilon => nfa.pushNode (.epsilon next) (by simp [Node.inBounds]; exact Nat.lt_trans next.isLt (Nat.lt_succ_self _))
+  | .char c => nfa.pushNode (.char c next) (by simp [Node.inBounds]; exact Nat.lt_trans next.isLt (Nat.lt_succ_self _))
+  | .alternate r₁ r₂ =>
+    -- TODO: it feels better to compile r₂ first to align with concat
+    let nfa₁ := nfa.pushRegex next r₁
+    let start₁ := nfa₁.val.start
+    let nfa₂ := nfa₁.val.pushRegex ⟨next, Nat.lt_trans next.isLt nfa₁.property⟩ r₂
+    let start₂ := nfa₂.val.start
+
+    let split := Node.split start₁ start₂
+    have inBounds : split.inBounds (nfa₂.val.nodes.size + 1) := by
+      have lt₁ : start₁ < nfa₂.val.nodes.size + 1 :=
+        calc
+          _ < _ := start₁.isLt
+          _ < _ := nfa₂.property
+          _ < _ := Nat.lt_succ_self _
+      have lt₂ : start₂ < nfa₂.val.nodes.size + 1 := Nat.lt_trans start₂.isLt (Nat.lt_succ_self _)
+      simp [lt₁, lt₂]
+
+    let nfa' := nfa₂.val.pushNode split inBounds
+    have property : nfa.nodes.size < nfa'.val.nodes.size :=
+      calc
+        _ < _ := nfa₁.property
+        _ < _ := nfa₂.property
+        _ < _ := nfa'.property
+
+    ⟨nfa', property⟩
+  | .concat r₁ r₂ =>
+    let nfa₂ := nfa.pushRegex next r₂
+    let nfa₁ := nfa₂.val.pushRegex nfa₂.val.start r₁
+
+    ⟨nfa₁, Nat.lt_trans nfa₂.property nfa₁.property⟩
+  | .star r =>
+    -- We need to generate a placeholder node first. We use `fail` for it because
+    -- 1. We'll use the fact that `fail` is a minimal element when strengthening induction hypotheis;
+    -- 2. We want to make sure `done` does not appear except at the first node.
+    -- 3. variants without data are represented as a boxed integer so there is one less allocation.
+    let placeholder := nfa.pushNode .fail rfl
+    let loopStart := placeholder.val.start
+    -- FIXME: generated code keeps `placeholder` alive, copying the array. Why?
+    let compiled := placeholder.val.pushRegex loopStart r
+
+    -- Patch the placeholder node
+    have isLt : loopStart.val < compiled.val.nodes.size :=
+      calc
+        _ < _ := loopStart.isLt
+        _ < _ := compiled.property
+    let loopStart := ⟨loopStart.val, isLt⟩
+
+    let split := Node.split compiled.val.start next
+    let patched := compiled.val.nodes.set loopStart split
+    have inBounds := by
+      -- Somehow putting the type directly on `inBounds` causes an infinite loop
+      show ∀ i : Fin patched.size, patched[i].inBounds patched.size
+      -- FIXME: I don't know how to unfold only `patched`
+      show ∀ i : Fin (compiled.val.nodes.set loopStart split).size, (compiled.val.nodes.set loopStart split)[i].inBounds (compiled.val.nodes.set loopStart split).size
+      intro i
+      have hj : i < compiled.val.nodes.size := by
+        suffices i.val < (compiled.val.nodes.set loopStart split).size by
+          -- Bare simp expands `let` declarations
+          simp (config := {zeta := false}) at this
+          exact this
+        exact i.isLt
+      rw [getElem_fin, Array.get_set (hj := hj)]
+      split
+      case inl =>
+        have lt₁ : compiled.val.start < compiled.val.nodes.size := compiled.val.start.isLt
+        have lt₂ : next < compiled.val.nodes.size :=
+          calc
+            _ < _ := next.isLt
+            _ < _ := placeholder.property
+            _ < _ := compiled.property
+        simp [lt₁, lt₂]
+      case inr neq =>
+        have := compiled.val.inBounds ⟨i, hj⟩
+        simp (config := {zeta := false}) at this
+        simp (config := {zeta := false})
+        simp [this]
+
+    let nfa' := ⟨patched, loopStart.cast (by rw [Array.size_set]), inBounds⟩
+    have property :=
+      calc
+        _ < _ := placeholder.property
+        _ < _ := compiled.property
+        _ = nfa'.nodes.size := by simp
+
+    ⟨nfa', property⟩
+
+-- TODO: push .*? for search
+def compile (r : Regex) : NFAa := done.pushRegex ⟨0, by decide⟩ r
+
+-- Useful lemmas about the compilation
+theorem pushRegex.empty (eq : pushRegex nfa next .empty = result)
+  {motive : result = nfa.pushNode .fail rfl → P} : P := by
+  simp [pushRegex] at eq
+  exact motive eq.symm
+
+theorem pushRegex.epsilon (eq : pushRegex nfa next .epsilon = result)
+  {motive : result = nfa.pushNode (.epsilon next) (by simp [Node.inBounds]; exact Nat.lt_trans next.isLt (Nat.lt_succ_self _)) → P} : P := by
+  simp [pushRegex] at eq
+  exact motive eq.symm
+
+theorem pushRegex.char (eq : pushRegex nfa next (.char c) = result)
+  {motive : result = nfa.pushNode (.char c next) (by simp [Node.inBounds]; exact Nat.lt_trans next.isLt (Nat.lt_succ_self _)) → P} : P := by
+  simp [pushRegex] at eq
+  exact motive eq.symm
+
+theorem pushRegex.alternate (eq : pushRegex nfa next (Regex.alternate r₁ r₂) = result)
+  {motive : ∀ nfa₁ start₁ nfa₂ start₂ inBounds nfa' property,
+    nfa₁ = nfa.pushRegex next r₁ →
+    start₁ = nfa₁.val.start →
+    nfa₂ = nfa₁.val.pushRegex ⟨next, Nat.lt_trans next.isLt nfa₁.property⟩ r₂ →
+    start₂ = nfa₂.val.start →
+    nfa' = nfa₂.val.pushNode (.split start₁ start₂) inBounds →
+    result = ⟨nfa', property⟩ →
+    P
+  } : P := by
+  let nfa₁ := nfa.pushRegex next r₁
+  let start₁ := nfa₁.val.start
+  let nfa₂ := nfa₁.val.pushRegex ⟨next, Nat.lt_trans next.isLt nfa₁.property⟩ r₂
+  let start₂ := nfa₂.val.start
+
+  let split := Node.split start₁ start₂
+  have inBounds : split.inBounds (nfa₂.val.nodes.size + 1) := by
+    have lt₁ : start₁ < nfa₂.val.nodes.size + 1 :=
+      calc
+        _ < _ := start₁.isLt
+        _ < _ := nfa₂.property
+        _ < _ := Nat.lt_succ_self _
+    have lt₂ : start₂ < nfa₂.val.nodes.size + 1 := Nat.lt_trans start₂.isLt (Nat.lt_succ_self _)
+    simp [lt₁, lt₂]
+
+  let nfa' := nfa₂.val.pushNode split inBounds
+  have property : nfa.nodes.size < nfa'.val.nodes.size :=
+    calc
+      _ < _ := nfa₁.property
+      _ < _ := nfa₂.property
+      _ < _ := nfa'.property
+
+  exact motive nfa₁ start₁ nfa₂ start₂ inBounds nfa' property rfl rfl rfl rfl rfl eq.symm
+
+theorem pushRegex.concat (eq : pushRegex nfa next (Regex.concat r₁ r₂) = result)
+  {motive : ∀ nfa₂ nfa₁ property,
+    nfa₂ = nfa.pushRegex next r₂ →
+    nfa₁ = nfa₂.val.pushRegex nfa₂.val.start r₁ →
+    result = ⟨nfa₁, property⟩ →
+    P
+  } : P := by
+  let nfa₂ := nfa.pushRegex next r₂
+  let nfa₁ := nfa₂.val.pushRegex nfa₂.val.start r₁
+
+  have property : nfa.nodes.size < nfa₁.val.nodes.size :=
+    calc
+      _ < _ := nfa₂.property
+      _ < _ := nfa₁.property
+
+  exact motive nfa₂ nfa₁ property rfl rfl eq.symm
+
+theorem pushRegex.star (eq : pushRegex nfa next (Regex.star r) = result)
+  {motive : ∀ placeholder compiled patched nfa' isLt inBounds property,
+    placeholder = nfa.pushNode .fail rfl →
+    compiled = placeholder.val.pushRegex ⟨nfa.nodes.size, placeholder.property⟩ r →
+    patched = compiled.val.nodes.set
+      ⟨nfa.nodes.size, Nat.lt_trans placeholder.property compiled.property⟩
+      (Node.split compiled.val.start next) →
+    nfa' = ⟨patched, ⟨nfa.nodes.size, isLt⟩, inBounds⟩ →
+    result = ⟨nfa', property⟩ →
+    P
+  } : P := by
+  let placeholder := nfa.pushNode .fail rfl
+  let compiled := placeholder.val.pushRegex ⟨nfa.nodes.size, placeholder.property⟩ r
+
+  -- Patch the placeholder node
+  let loopStart : Fin _ := ⟨nfa.nodes.size, Nat.lt_trans placeholder.property compiled.property⟩
+  let split := Node.split compiled.val.start next
+  let patched := compiled.val.nodes.set loopStart split
+  have inBounds := by
+    -- Somehow putting the type directly on `inBounds` causes an infinite loop
+    show ∀ i : Fin patched.size, patched[i].inBounds patched.size
+    -- FIXME: I don't know how to unfold only `patched`
+    show ∀ i : Fin (compiled.val.nodes.set loopStart split).size, (compiled.val.nodes.set loopStart split)[i].inBounds (compiled.val.nodes.set loopStart split).size
+    intro i
+    have hj : i < compiled.val.nodes.size := by
+      suffices i.val < (compiled.val.nodes.set loopStart split).size by
+        -- Bare simp expands `let` declarations
+        simp (config := {zeta := false}) at this
+        exact this
+      exact i.isLt
+    rw [getElem_fin, Array.get_set (hj := hj)]
+    split
+    case inl =>
+      have lt₁ : compiled.val.start < compiled.val.nodes.size := compiled.val.start.isLt
+      have lt₂ : next < compiled.val.nodes.size :=
+        calc
+          _ < _ := next.isLt
+          _ < _ := placeholder.property
+          _ < _ := compiled.property
+      simp [lt₁, lt₂]
+    case inr neq =>
+      have := compiled.val.inBounds ⟨i, hj⟩
+      simp (config := {zeta := false}) at this
+      simp (config := {zeta := false})
+      simp [this]
+
+  have isLt : nfa.nodes.size < patched.size :=
+    calc
+      _ < _ := placeholder.property
+      _ < _ := compiled.property
+      _ = _ := by simp
+  let nfa' : NFAa := ⟨patched, ⟨nfa.nodes.size, isLt⟩, inBounds⟩
+  have property :=
+    calc
+      _ < _ := placeholder.property
+      _ < _ := compiled.property
+      _ = nfa'.nodes.size := by simp
+
+  exact motive placeholder compiled patched nfa' isLt inBounds property rfl rfl rfl rfl eq.symm
+
+end NFAa
+
 namespace NFA
 
 def NFA.addNode (nfa : NFA) (node : Node) :
