Regex/NFA/VM/Basic.lean
@@ -403,6 +403,72 @@ where
       go nfa inBounds c init accum (i + 1) hlt
 termination_by go _ => nfa.nodes.size - i
 
+-- TODO: check if the modifications don't cause copying
+def εClosureTRa (nfa : NFAa) (visited : NodeSet nfa.nodes.size) (stack : Array (Fin nfa.nodes.size)) :
+  NodeSet nfa.nodes.size :=
+  if hemp : stack.isEmpty then
+    visited
+  else
+    let i := stack.back' hemp
+    let stack' := stack.pop
+    have : stack'.size < stack.size := Array.lt_size_of_pop_of_not_empty _ hemp
+    if hvis : visited.get i then
+      εClosureTRa nfa visited stack'
+    else
+      let visited' := visited.set i
+      have : visited'.count_unset < visited.count_unset := visited.lt_count_unset i.isLt hvis
+      have inBounds' := nfa.inBounds i
+      let stack'' :=
+        match hn : nfa.nodes[i.val] with
+        | .epsilon next =>
+          have h : next < nfa.nodes.size := by
+            rw [hn] at inBounds'
+            simp [Node.inBounds] at inBounds'
+            exact inBounds'
+
+          stack'.push ⟨next, h⟩
+        | .split next₁ next₂ =>
+          have h₁ : next₁ < nfa.nodes.size := by
+            rw [hn] at inBounds'
+            simp [Node.inBounds] at inBounds'
+            exact inBounds'.left
+          have h₂ : next₂ < nfa.nodes.size := by
+            rw [hn] at inBounds'
+            simp [Node.inBounds] at inBounds'
+            exact inBounds'.right
+
+          (stack'.push ⟨next₁, h₁⟩).push ⟨next₂, h₂⟩
+        | _ => stack'
+      εClosureTRa nfa visited' stack''
+termination_by _ => (visited.count_unset, stack.size)
+
+def charStepTRa (nfa : NFAa) (c : Char) (init : NodeSet nfa.nodes.size) :
+  NodeSet nfa.nodes.size := go nfa c init .empty 0 (Nat.zero_le _)
+where
+  go (nfa : NFAa) (c : Char) (init : NodeSet nfa.nodes.size)
+    (accum : NodeSet nfa.nodes.size) (i : Nat) (hle : i ≤ nfa.nodes.size) :
+    NodeSet nfa.nodes.size :=
+    if h : i = nfa.nodes.size then
+      accum
+    else
+      have hlt : i < nfa.nodes.size := Nat.lt_of_le_of_ne hle h
+      let accum := if init.get ⟨i, hlt⟩ then
+        match hn : nfa.nodes[i] with
+        | .char c' next =>
+          if c = c' then
+            have : next < nfa.nodes.size := by
+              have := nfa.inBounds ⟨i, hlt⟩
+              simp [hn, Node.inBounds] at this
+              exact this
+            -- TODO: reuse visited and stack
+            accum.merge (εClosureTRa nfa .empty #[⟨next, this⟩])
+          else
+            accum
+        | _ => accum
+      else accum
+      go nfa c init accum (i + 1) hlt
+termination_by go _ => nfa.nodes.size - i
+
 end NFA.VM
 
 open NFA.VM
@@ -420,3 +486,16 @@ where
     else
       let ns' := charStepTR nfa inBounds iter.curr ns
       go nfa inBounds iter.next ns'
+
+def NFAa.match (nfa : NFAa) (s : String) : Bool :=
+  let ns := εClosureTRa nfa .empty #[nfa.start]
+  let ns := go nfa s.iter ns
+  -- This assumes that the first node is the accepting node
+  ns.get ⟨0, nfa.zero_lt_size⟩
+where
+  go (nfa : NFAa) (iter : String.Iterator) (ns : NodeSet nfa.nodes.size) : NodeSet nfa.nodes.size :=
+    if iter.atEnd then
+      ns
+    else
+      let ns' := charStepTRa nfa iter.curr ns
+      go nfa iter.next ns'
