Regex/NFA/Tests.lean
@@ -2,28 +2,24 @@ import Regex.NFA.Compile
 import Regex.NFA.VM
 
 def r₁ := Regex.concat (Regex.star (Regex.char 'a')) (Regex.star (Regex.char 'b'))
-def NFA₁ := NFA.compile r₁
-def inBounds₁ : NFA₁.inBounds := NFA.compile.inBounds rfl
-#eval NFA₁.match inBounds₁ "aaaabbbb"
-#eval NFA₁.match inBounds₁ "ab"
-#eval NFA₁.match inBounds₁ "c"
-#eval NFA₁.match inBounds₁ ""
+def NFA₁ := NFAa.compile r₁
+#eval NFA₁.match "aaaabbbb"
+#eval NFA₁.match "ab"
+#eval NFA₁.match "c"
+#eval NFA₁.match ""
 
 def r₂ := Regex.star (Regex.alternate (Regex.star (Regex.char 'a')) (Regex.char 'b'))
-def NFA₂ := NFA.compile r₂
-def inBounds₂ : NFA₂.inBounds := NFA.compile.inBounds rfl
-#eval NFA₂.match inBounds₂ "aaaabbbb"
-#eval NFA₂.match inBounds₂ "abcab"
-#eval NFA₂.match inBounds₂ ""
+def NFA₂ := NFAa.compile r₂
+#eval NFA₂.match "aaaabbbb"
+#eval NFA₂.match "abcab"
+#eval NFA₂.match ""
 
-def NFA₃ := NFA.compile (Regex.alternate Regex.empty (Regex.concat (Regex.char 'a') Regex.empty))
-def inBounds₃ : NFA₃.inBounds := NFA.compile.inBounds rfl
-#eval NFA₃.match inBounds₃ ""
-#eval NFA₃.match inBounds₃ "a"
+def NFA₃ := NFAa.compile (Regex.alternate Regex.empty (Regex.concat (Regex.char 'a') Regex.empty))
+#eval NFA₃.match ""
+#eval NFA₃.match "a"
 
-def NFA₄ := NFA.compile (Regex.concat (Regex.alternate (Regex.char 'a') (Regex.char 'b')) (Regex.char 'c'))
-def inBounds₄ : NFA₄.inBounds := NFA.compile.inBounds rfl
-#eval NFA₄.match inBounds₄ "ac"
-#eval NFA₄.match inBounds₄ "bc"
-#eval NFA₄.match inBounds₄ "a"
-#eval NFA₄.match inBounds₄ ""
+def NFA₄ := NFAa.compile (Regex.concat (Regex.alternate (Regex.char 'a') (Regex.char 'b')) (Regex.char 'c'))
+#eval NFA₄.match "ac"
+#eval NFA₄.match "bc"
+#eval NFA₄.match "a"
+#eval NFA₄.match ""
